[APT] Improve the TAILREC transormation.
Now the automatically generated names for the new and wrapper function (when
:NEW-NAME is :AUTO and/or :WRAPPER-NAME is :AUTO) are as follows. If the wrapper
is not generated, the new name is obtained by adding or suitably incrementing
the explicit or implicit index of tha target function; this is as before. But if
the wrapper is generated, then that name is used for the wrapper, while the new
function has the form ...-AUX{...}, as common when a function (the wrapper in
this case) needs a "loop". The conjecture behind this change is that most of the
time we do not generate the wrapper, unless the function being transformed is
one of the top-level functions, in which case we want the wrapper, which has the
same interface as the target function, and we want it to have a name that
relates directly to the old function. This approach may be revisited in the
future. Also, in the future we may support more flexible naming schemes than the
form ...-AUX{...} for the generated tail-recursive function when there is a
wrapper.

Update the user documentation accordingly.

Update some tests accordingtly.

books/kestrel/apt/tailrec-tests.lisp
@@ -13,7 +13,10 @@
 (include-book "tailrec")
 
 (include-book "std/testing/assert-bang" :dir :system)
-(include-book "std/testing/eval" :dir :system)
+(include-book "std/testing/must-be-redundant" :dir :system)
+(include-book "std/testing/must-fail" :dir :system)
+(include-book "std/testing/must-fail-local" :dir :system)
+(include-book "std/testing/must-succeed-star" :dir :system)
 
 ;;;;;;;;;;;;;;;;;;;;;;;;;;;;;;;;;;;;;;;;;;;;;;;;;;;;;;;;;;;;;;;;;;;;;;;;;;;;;;;;
 
@@ -166,11 +169,11 @@
   (defun f (x) (if (atom x) nil (lub (car x) (f (cdr x)))))
   (tailrec f)
   (must-be-redundant
-   (defun f{1} (x r)
+   (defun f-aux{1} (x r)
      (declare (xargs :measure (acl2-count x)))
-     (if (atom x) r (f{1} (cdr x) (lub r (car x)))))
-   (defun f{1}-wrapper (x) (f{1} x nil))
-   (defthm f-~>-f{1}-wrapper (equal (f x) (f{1}-wrapper x)))))
+     (if (atom x) r (f-aux{1} (cdr x) (lub r (car x)))))
+   (defun f{1} (x) (f-aux{1} x nil))
+   (defthm f-~>-f{1} (equal (f x) (f{1} x)))))
 
  ;; without guard verification:
  (must-succeed*
@@ -179,13 +182,13 @@
     (if (atom x) nil (lub (car x) (f (cdr x)))))
   (tailrec f)
   (must-be-redundant
-   (defun f{1} (x r)
+   (defun f-aux{1} (x r)
      (declare (xargs :measure (acl2-count x) :verify-guards nil))
-     (if (atom x) r (f{1} (cdr x) (lub r (car x)))))
-   (defun f{1}-wrapper (x)
+     (if (atom x) r (f-aux{1} (cdr x) (lub r (car x)))))
+   (defun f{1} (x)
      (declare (xargs :verify-guards nil))
-     (f{1} x nil))
-   (defthm f-~>-f{1}-wrapper (equal (f x) (f{1}-wrapper x))))))
+     (f-aux{1} x nil))
+   (defthm f-~>-f{1} (equal (f x) (f{1} x))))))
 
 ;;;;;;;;;;;;;;;;;;;;;;;;;;;;;;;;;;;;;;;;;;;;;;;;;;;;;;;;;;;;;;;;;;;;;;;;;;;;;;;;
 
@@ -211,41 +214,41 @@
  (must-succeed*
   (tailrec f)
   (must-be-redundant
-   (defun f{1} (x r)
+   (defun f-aux{1} (x r)
      (declare (xargs :measure (acl2-count x)))
-     (if (atom x) r (f{1} (cdr x) (lub r (car x)))))
-   (defun f{1}-wrapper (x) (f{1} x nil))
-   (defthm f-~>-f{1}-wrapper (equal (f x) (f{1}-wrapper x)))))
+     (if (atom x) r (f-aux{1} (cdr x) (lub r (car x)))))
+   (defun f{1} (x) (f-aux{1} x nil))
+   (defthm f-~>-f{1} (equal (f x) (f{1} x)))))
 
  ;; monoidal:
  (must-succeed*
   (tailrec f :variant :monoid)
   (must-be-redundant
-   (defun f{1} (x r)
+   (defun f-aux{1} (x r)
      (declare (xargs :measure (acl2-count x)))
-     (if (atom x) r (f{1} (cdr x) (lub r (car x)))))
-   (defun f{1}-wrapper (x) (f{1} x nil))
-   (defthm f-~>-f{1}-wrapper (equal (f x) (f{1}-wrapper x)))))
+     (if (atom x) r (f-aux{1} (cdr x) (lub r (car x)))))
+   (defun f{1} (x) (f-aux{1} x nil))
+   (defthm f-~>-f{1} (equal (f x) (f{1} x)))))
 
  ;; alternative monoidal:
  (must-succeed*
   (tailrec f :variant :monoid-alt)
   (must-be-redundant
-   (defun f{1} (x r)
+   (defun f-aux{1} (x r)
      (declare (xargs :measure (acl2-count x)))
-     (if (atom x) r (f{1} (cdr x) (lub r (car x)))))
-   (defun f{1}-wrapper (x) (f{1} x nil))
-   (defthm f-~>-f{1}-wrapper (equal (f x) (f{1}-wrapper x)))))
+     (if (atom x) r (f-aux{1} (cdr x) (lub r (car x)))))
+   (defun f{1} (x) (f-aux{1} x nil))
+   (defthm f-~>-f{1} (equal (f x) (f{1} x)))))
 
  ;; associative:
  (must-succeed*
   (tailrec f :variant :assoc)
   (must-be-redundant
-   (defun f{1} (x r)
+   (defun f-aux{1} (x r)
      (declare (xargs :measure (acl2-count x)))
-     (if (atom x) (lub r nil) (f{1} (cdr x) (lub r (car x)))))
-   (defun f{1}-wrapper (x) (and (not (atom x)) (f{1} (cdr x) (car x))))
-   (defthm f-~>-f{1}-wrapper (equal (f x) (f{1}-wrapper x))))))
+     (if (atom x) (lub r nil) (f-aux{1} (cdr x) (lub r (car x)))))
+   (defun f{1} (x) (and (not (atom x)) (f-aux{1} (cdr x) (car x))))
+   (defthm f-~>-f{1} (equal (f x) (f{1} x))))))
 
 ;;;;;;;;;;;;;;;;;;;;;;;;;;;;;;;;;;;;;;;;;;;;;;;;;;;;;;;;;;;;;;;;;;;;;;;;;;;;;;;;
 
@@ -323,66 +326,66 @@
   (must-succeed*
    (tailrec fact)
    (must-be-redundant
-    (defun fact{1} (n r)
+    (defun fact-aux{1} (n r)
       (declare (xargs :measure (acl2-count n)
                       :guard (and (natp n) (acl2-numberp r))))
-      (if (zp n) r (fact{1} (+ -1 n) (* r n))))
-    (defun fact{1}-wrapper (n)
+      (if (zp n) r (fact-aux{1} (+ -1 n) (* r n))))
+    (defun fact{1} (n)
       (declare (xargs :guard (natp n)))
-      (fact{1} n 1))
-    (defthm fact-~>-fact{1}-wrapper (equal (fact n) (fact{1}-wrapper n)))))
+      (fact-aux{1} n 1))
+    (defthm fact-~>-fact{1} (equal (fact n) (fact{1} n)))))
 
   ;; automatic:
   (must-succeed*
    (tailrec fact :domain :auto)
    (must-be-redundant
-    (defun fact{1} (n r)
+    (defun fact-aux{1} (n r)
       (declare (xargs :measure (acl2-count n)
                       :guard (and (natp n) (acl2-numberp r))))
-      (if (zp n) r (fact{1} (+ -1 n) (* r n))))
-    (defun fact{1}-wrapper (n)
+      (if (zp n) r (fact-aux{1} (+ -1 n) (* r n))))
+    (defun fact{1} (n)
       (declare (xargs :guard (natp n)))
-      (fact{1} n 1))
-    (defthm fact-~>-fact{1}-wrapper (equal (fact n) (fact{1}-wrapper n)))))
+      (fact-aux{1} n 1))
+    (defthm fact-~>-fact{1} (equal (fact n) (fact{1} n)))))
 
   ;; function name:
   (must-succeed*
    (tailrec fact :domain natp)
    (must-be-redundant
-    (defun fact{1} (n r)
+    (defun fact-aux{1} (n r)
       (declare (xargs :measure (acl2-count n) :guard (and (natp n) (natp r))))
-      (if (zp n) r (fact{1} (+ -1 n) (* r n))))
-    (defun fact{1}-wrapper (n)
+      (if (zp n) r (fact-aux{1} (+ -1 n) (* r n))))
+    (defun fact{1} (n)
       (declare (xargs :guard (natp n)))
-      (fact{1} n 1))
-    (defthm fact-~>-fact{1}-wrapper (equal (fact n) (fact{1}-wrapper n)))))
+      (fact-aux{1} n 1))
+    (defthm fact-~>-fact{1} (equal (fact n) (fact{1} n)))))
 
   ;; macro name:
   (must-succeed*
    (defmacro intp (m) `(integerp ,m))
    (tailrec fact :domain intp)
    (must-be-redundant
-    (defun fact{1} (n r)
+    (defun fact-aux{1} (n r)
       (declare (xargs :measure (acl2-count n)
                       :guard (and (natp n) (integerp r))))
-      (if (zp n) r (fact{1} (+ -1 n) (* r n))))
-    (defun fact{1}-wrapper (n)
+      (if (zp n) r (fact-aux{1} (+ -1 n) (* r n))))
+    (defun fact{1} (n)
       (declare (xargs :guard (natp n)))
-      (fact{1} n 1))
-    (defthm fact-~>-fact{1}-wrapper (equal (fact n) (fact{1}-wrapper n)))))
+      (fact-aux{1} n 1))
+    (defthm fact-~>-fact{1} (equal (fact n) (fact{1} n)))))
 
   ;; lambda expression:
   (must-succeed*
    (tailrec fact :domain (lambda (a) (acl2-numberp a)))
    (must-be-redundant
-    (defun fact{1} (n r)
+    (defun fact-aux{1} (n r)
       (declare (xargs :measure (acl2-count n)
                       :guard (and (natp n) (acl2-numberp r))))
-      (if (zp n) r (fact{1} (+ -1 n) (* r n))))
-    (defun fact{1}-wrapper (n)
+      (if (zp n) r (fact-aux{1} (+ -1 n) (* r n))))
+    (defun fact{1} (n)
       (declare (xargs :guard (natp n)))
-      (fact{1} n 1))
-    (defthm fact-~>-fact{1}-wrapper (equal (fact n) (fact{1}-wrapper n)))))))
+      (fact-aux{1} n 1))
+    (defthm fact-~>-fact{1} (equal (fact n) (fact{1} n)))))))
 
 ;;;;;;;;;;;;;;;;;;;;;;;;;;;;;;;;;;;;;;;;;;;;;;;;;;;;;;;;;;;;;;;;;;;;;;;;;;;;;;;;
 
@@ -416,12 +419,12 @@
  ;; default:
  (must-succeed*
   (tailrec f)
-  (assert! (function-namep 'f{1} (w state))))
+  (assert! (function-namep 'f-aux{1} (w state))))
 
  ;; automatic:
  (must-succeed*
   (tailrec f :new-name :auto)
-  (assert! (function-namep 'f{1} (w state))))
+  (assert! (function-namep 'f-aux{1} (w state))))
 
  ;; specified:
  (must-succeed*
@@ -451,46 +454,46 @@
  ;; default, with target function enabled:
  (must-succeed*
   (tailrec f)
-  (assert! (fundef-enabledp 'f{1} state)))
+  (assert! (fundef-enabledp 'f-aux{1} state)))
 
  ;; default, with target function disabled:
  (must-succeed*
   (in-theory (disable f))
   (tailrec f)
-  (assert! (fundef-disabledp 'f{1} state)))
+  (assert! (fundef-disabledp 'f-aux{1} state)))
 
  ;; automatic, with target function enabled:
  (must-succeed*
   (tailrec f :new-enable :auto)
-  (assert! (fundef-enabledp 'f{1} state)))
+  (assert! (fundef-enabledp 'f-aux{1} state)))
 
  ;; automatic, with target function disabled:
  (must-succeed*
   (in-theory (disable f))
   (tailrec f :new-enable :auto)
-  (assert! (fundef-disabledp 'f{1} state)))
+  (assert! (fundef-disabledp 'f-aux{1} state)))
 
  ;; enable, with target function enabled:
  (must-succeed*
   (tailrec f :new-enable t)
-  (assert! (fundef-enabledp 'f{1} state)))
+  (assert! (fundef-enabledp 'f-aux{1} state)))
 
  ;; enable, with target function disabled:
  (must-succeed*
   (in-theory (disable f))
   (tailrec f :new-enable t)
-  (assert! (fundef-enabledp 'f{1} state)))
+  (assert! (fundef-enabledp 'f-aux{1} state)))
 
  ;; disable, with target function enabled:
  (must-succeed*
   (tailrec f :new-enable nil)
-  (assert! (fundef-disabledp 'f{1} state)))
+  (assert! (fundef-disabledp 'f-aux{1} state)))
 
  ;; disable, with target function disabled:
  (must-succeed*
   (in-theory (disable f))
   (tailrec f :new-enable nil)
-  (assert! (fundef-disabledp 'f{1} state))))
+  (assert! (fundef-disabledp 'f-aux{1} state))))
 
 ;;;;;;;;;;;;;;;;;;;;;;;;;;;;;;;;;;;;;;;;;;;;;;;;;;;;;;;;;;;;;;;;;;;;;;;;;;;;;;;;
 
@@ -515,17 +518,20 @@
  ;; default:
  (must-succeed*
   (tailrec f)
-  (assert! (function-namep 'f{1}-wrapper (w state))))
+  (assert! (function-namep 'f{1} (w state)))
+  (assert! (not (irecursivep 'f{1} (w state)))))
 
  ;; generate:
  (must-succeed*
   (tailrec f :wrapper t)
-  (assert! (function-namep 'f{1}-wrapper (w state))))
+  (assert! (function-namep 'f{1} (w state)))
+  (assert! (not (irecursivep 'f{1} (w state)))))
 
  ;; do not generate:
  (must-succeed*
   (tailrec f :wrapper nil)
-  (assert! (not (function-namep 'f{1}-wrapper (w state))))))
+  (assert! (function-namep 'f{1} (w state)))
+  (assert! (irecursivep 'f{1} (w state)))))
 
 ;;;;;;;;;;;;;;;;;;;;;;;;;;;;;;;;;;;;;;;;;;;;;;;;;;;;;;;;;;;;;;;;;;;;;;;;;;;;;;;;
 
@@ -559,12 +565,12 @@
  ;; default:
  (must-succeed*
   (tailrec f)
-  (assert! (function-namep 'f{1}-wrapper (w state))))
+  (assert! (function-namep 'f{1} (w state))))
 
  ;; automatic:
  (must-succeed*
   (tailrec f :wrapper-name :auto)
-  (assert! (function-namep 'f{1}-wrapper (w state))))
+  (assert! (function-namep 'f{1} (w state))))
 
  ;; specified:
  (must-succeed*
@@ -594,17 +600,17 @@
  ;; default:
  (must-succeed*
   (tailrec f)
-  (assert! (fundef-enabledp 'f{1}-wrapper state)))
+  (assert! (fundef-enabledp 'f{1} state)))
 
  ;; enable:
  (must-succeed*
   (tailrec f :wrapper-enable t)
-  (assert! (fundef-enabledp 'f{1}-wrapper state)))
+  (assert! (fundef-enabledp 'f{1} state)))
 
  ;; disable:
  (must-succeed*
   (tailrec f :wrapper-enable nil)
-  (assert! (fundef-disabledp 'f{1}-wrapper state))))
+  (assert! (fundef-disabledp 'f{1} state))))
 
 ;;;;;;;;;;;;;;;;;;;;;;;;;;;;;;;;;;;;;;;;;;;;;;;;;;;;;;;;;;;;;;;;;;;;;;;;;;;;;;;;
 
@@ -637,23 +643,23 @@
 
  ;; determining a name that already exists:
  (must-succeed*
-  (defun f-is-f{1}-wrapper () nil)
+  (defun f-is-f{1} () nil)
   (must-fail (tailrec f :thm-name :is)))
 
  ;; determining, by default, a name that already exists:
  (must-succeed*
-  (defun f-~>-f{1}-wrapper () nil)
+  (defun f-~>-f{1} () nil)
   (must-fail (tailrec f)))
 
  ;; default:
  (must-succeed*
   (tailrec f)
-  (assert! (theorem-namep 'f-~>-f{1}-wrapper (w state))))
+  (assert! (theorem-namep 'f-~>-f{1} (w state))))
 
  ;; automatic:
  (must-succeed*
   (tailrec f :thm-name :auto)
-  (assert! (theorem-namep 'f-~>-f{1}-wrapper (w state))))
+  (assert! (theorem-namep 'f-~>-f{1} (w state))))
 
  ;; specified:
  (must-succeed*
@@ -683,17 +689,17 @@
  ;; default:
  (must-succeed*
   (tailrec f)
-  (assert! (rune-enabledp '(:rewrite f-~>-f{1}-wrapper) state)))
+  (assert! (rune-enabledp '(:rewrite f-~>-f{1}) state)))
 
  ;; enable:
  (must-succeed*
   (tailrec f :thm-enable t)
-  (assert! (rune-enabledp '(:rewrite f-~>-f{1}-wrapper) state)))
+  (assert! (rune-enabledp '(:rewrite f-~>-f{1}) state)))
 
  ;; disable:
  (must-succeed*
   (tailrec f :thm-enable nil)
-  (assert! (rune-disabledp '(:rewrite f-~>-f{1}-wrapper) state))))
+  (assert! (rune-disabledp '(:rewrite f-~>-f{1}) state))))
 
 ;;;;;;;;;;;;;;;;;;;;;;;;;;;;;;;;;;;;;;;;;;;;;;;;;;;;;;;;;;;;;;;;;;;;;;;;;;;;;;;;
 
@@ -719,14 +725,14 @@
 
  ;; transforming F preserves executability:
  (tailrec f)
+ (assert! (not (non-executablep 'f-aux{1} (w state))))
  (assert! (not (non-executablep 'f{1} (w state))))
- (assert! (not (non-executablep 'f{1}-wrapper (w state))))
 
  ;; transforming G preserves non-executability:
  (tailrec g)
- (assert! (non-executablep 'g{1} (w state)))
+ (assert! (non-executablep 'g-aux{1} (w state)))
  ;; but the wrapper is always executable:
- (assert! (not (non-executablep 'g{1}-wrapper (w state)))))
+ (assert! (not (non-executablep 'g{1} (w state)))))
 
 ;;;;;;;;;;;;;;;;;;;;;;;;;;;;;;;;;;;;;;;;;;;;;;;;;;;;;;;;;;;;;;;;;;;;;;;;;;;;;;;;
 
@@ -757,27 +763,27 @@
  ;; default, with target function guard-verified:
  (must-succeed*
   (tailrec f)
-  (assert! (guard-verified-p 'f{1} (w state))))
+  (assert! (guard-verified-p 'f-aux{1} (w state))))
 
  ;; default, with target function not guard-verified:
  (must-succeed*
   (tailrec g)
-  (assert! (not (guard-verified-p 'g{1} (w state)))))
+  (assert! (not (guard-verified-p 'g-aux{1} (w state)))))
 
  ;; automatic, with target function guard-verified:
  (must-succeed*
   (tailrec f :verify-guards :auto)
-  (assert! (guard-verified-p 'f{1} (w state))))
+  (assert! (guard-verified-p 'f-aux{1} (w state))))
 
  ;; automatic, with target function not guard-verified:
  (must-succeed*
   (tailrec g :verify-guards :auto)
-  (assert! (not (guard-verified-p 'g{1} (w state)))))
+  (assert! (not (guard-verified-p 'g-aux{1} (w state)))))
 
  ;; verify guards, with target function guard-verified:
  (must-succeed*
   (tailrec f :verify-guards t)
-  (assert! (guard-verified-p 'f{1} (w state))))
+  (assert! (guard-verified-p 'f-aux{1} (w state))))
 
  ;; verify guards, with target function not guard-verified:
  (must-succeed*
@@ -786,12 +792,12 @@
  ;; do not verify guards, with target function guard-verified:
  (must-succeed*
   (tailrec f :verify-guards nil)
-  (assert! (not (guard-verified-p 'f{1} (w state)))))
+  (assert! (not (guard-verified-p 'f-aux{1} (w state)))))
 
  ;; do not verify guards, with target function not guard-verified:
  (must-succeed*
   (tailrec g :verify-guards nil)
-  (assert! (not (guard-verified-p 'g{1} (w state))))))
+  (assert! (not (guard-verified-p 'g-aux{1} (w state))))))
 
 ;;;;;;;;;;;;;;;;;;;;;;;;;;;;;;;;;;;;;;;;;;;;;;;;;;;;;;;;;;;;;;;;;;;;;;;;;;;;;;;;
 
@@ -920,18 +926,18 @@
  ;; default:
  (must-succeed*
   (tailrec f)
-  (assert! (function-namep 'f{1} (w state))))
+  (assert! (function-namep 'f-aux{1} (w state))))
 
  ;; show only:
  (must-succeed*
   (tailrec f :show-only t)
-  (assert! (not (function-namep 'f{1} (w state))))
+  (assert! (not (function-namep 'f-aux{1} (w state))))
   :with-output-off nil)
 
  ;; submit events:
  (must-succeed*
   (tailrec f :show-only nil)
-  (assert! (function-namep 'f{1} (w state))))
+  (assert! (function-namep 'f-aux{1} (w state))))
 
  :with-output-off nil)
 
@@ -1087,14 +1093,14 @@
     (if (zp n) 0 (+ n (tri (1- n)))))
   (tailrec tri :domain rationalp)
   (must-be-redundant
-   (defun tri{1} (n r)
+   (defun tri-aux{1} (n r)
      (declare (xargs :measure (acl2-count n)
                      :guard (and (natp n) (rationalp r))))
-     (if (zp n) r (tri{1} (+ -1 n) (+ r n))))
-   (defun tri{1}-wrapper (n)
+     (if (zp n) r (tri-aux{1} (+ -1 n) (+ r n))))
+   (defun tri{1} (n)
      (declare (xargs :guard (natp n)))
-     (tri{1} n 0))
-   (defthm tri-~>-tri{1}-wrapper (equal (tri n) (tri{1}-wrapper n)))))
+     (tri-aux{1} n 0))
+   (defthm tri-~>-tri{1} (equal (tri n) (tri{1} n)))))
 
  ;; pyramidal numbers (i.e. sum of squares):
  (must-succeed*
@@ -1103,14 +1109,14 @@
     (if (zp n) 0 (+ (* n n) (pyr (1- n)))))
   (tailrec pyr :domain integerp)
   (must-be-redundant
-   (defun pyr{1} (n r)
+   (defun pyr-aux{1} (n r)
      (declare (xargs :measure (acl2-count n)
                      :guard (and (natp n) (integerp r))))
-     (if (zp n) r (pyr{1} (+ -1 n) (+ r (* n n)))))
-   (defun pyr{1}-wrapper (n)
+     (if (zp n) r (pyr-aux{1} (+ -1 n) (+ r (* n n)))))
+   (defun pyr{1} (n)
      (declare (xargs :guard (natp n)))
-     (pyr{1} n 0))
-   (defthm pyr-~>-pyr{1}-wrapper (equal (pyr n) (pyr{1}-wrapper n)))))
+     (pyr-aux{1} n 0))
+   (defthm pyr-~>-pyr{1} (equal (pyr n) (pyr{1} n)))))
 
  ;; sum list elements:
  (must-succeed*
@@ -1119,15 +1125,15 @@
     (if (endp l) 0 (+ (car l) (list-sum (cdr l)))))
   (tailrec list-sum :variant :monoid-alt :domain acl2-numberp)
   (must-be-redundant
-   (defun list-sum{1} (l r)
+   (defun list-sum-aux{1} (l r)
      (declare (xargs :measure (acl2-count l)
                      :guard (and (acl2-number-listp l) (acl2-numberp r))))
-     (if (endp l) r (list-sum{1} (cdr l) (+ r (car l)))))
-   (defun list-sum{1}-wrapper (l)
+     (if (endp l) r (list-sum-aux{1} (cdr l) (+ r (car l)))))
+   (defun list-sum{1} (l)
      (declare (xargs :guard (acl2-number-listp l)))
-     (list-sum{1} l 0))
-   (defthm list-sum-~>-list-sum{1}-wrapper
-     (equal (list-sum l) (list-sum{1}-wrapper l)))))
+     (list-sum-aux{1} l 0))
+   (defthm list-sum-~>-list-sum{1}
+     (equal (list-sum l) (list-sum{1} l)))))
 
  ;; length of list:
  (must-succeed*
@@ -1136,15 +1142,15 @@
     (if (endp l) 0 (1+ (list-len (cdr l)))))
   (tailrec list-len :domain natp)
   (must-be-redundant
-   (defun list-len{1} (l r)
+   (defun list-len-aux{1} (l r)
      (declare (xargs :measure (acl2-count l)
                      :guard (and (true-listp l) (natp r))))
-     (if (endp l) r (list-len{1} (cdr l) (+ r 1))))
-   (defun list-len{1}-wrapper (l)
+     (if (endp l) r (list-len-aux{1} (cdr l) (+ r 1))))
+   (defun list-len{1} (l)
      (declare (xargs :guard (true-listp l)))
-     (list-len{1} l 0))
-   (defthm list-len-~>-list-len{1}-wrapper
-     (equal (list-len l) (list-len{1}-wrapper l)))))
+     (list-len-aux{1} l 0))
+   (defthm list-len-~>-list-len{1}
+     (equal (list-len l) (list-len{1} l)))))
 
  ;; reverse list:
  (must-succeed*
@@ -1152,12 +1158,12 @@
     (if (atom l) nil (append (list-rev (cdr l)) (list (car l)))))
   (tailrec list-rev :domain true-listp)
   (must-be-redundant
-   (defun list-rev{1} (l r)
+   (defun list-rev-aux{1} (l r)
      (declare (xargs :measure (acl2-count l) :guard (true-listp r)))
-     (if (atom l) r (list-rev{1} (cdr l) (append (list (car l)) r))))
-   (defun list-rev{1}-wrapper (l) (list-rev{1} l nil))
-   (defthm list-rev-~>-list-rev{1}-wrapper
-     (equal (list-rev l) (list-rev{1}-wrapper l)))))
+     (if (atom l) r (list-rev-aux{1} (cdr l) (append (list (car l)) r))))
+   (defun list-rev{1} (l) (list-rev-aux{1} l nil))
+   (defthm list-rev-~>-list-rev{1}
+     (equal (list-rev l) (list-rev{1} l)))))
 
  ;; raise to power:
  (must-succeed*
@@ -1166,13 +1172,13 @@
     (if (zp n) 1 (* x (power x (1- n)))))
   (tailrec power :variant :monoid-alt :domain acl2-numberp)
   (must-be-redundant
-   (defun power{1} (x n r)
+   (defun power-aux{1} (x n r)
      (declare (xargs :measure (acl2-count n)
                      :guard (and (and (acl2-numberp x) (natp n))
                                  (acl2-numberp r))))
-     (if (zp n) r (power{1} x (+ -1 n) (* r x))))
-   (defun power{1}-wrapper (x n)
+     (if (zp n) r (power-aux{1} x (+ -1 n) (* r x))))
+   (defun power{1} (x n)
      (declare (xargs :guard (and (acl2-numberp x) (natp n))))
-     (power{1} x n 1))
-   (defthm power-~>-power{1}-wrapper
-     (equal (power x n) (power{1}-wrapper x n))))))
+     (power-aux{1} x n 1))
+   (defthm power-~>-power{1}
+     (equal (power x n) (power{1} x n))))))
